Use `Type` instead of `go.type` for struct_field_ref, array_index_ref, etc.
This captures the fact that struct field offsets don't _actually_ depend
on the full go.type (e.g. go.uint64 or go.int64), but only on the
representation type (e.g. w64). This was implicitly what older versions
of Goose did via IntoVal encoding struct field offsets in flattened
struct/array values.

This avoids the need for go.type annotations in own_slice and for array
values.

Also add `TypeRepr` to map `t : go.type` to a `V : Type`. Might want to
bundle it into IntoValTyped at some point.

new/golang/defn/postlang.v
@@ -80,7 +80,12 @@ Class GoSemanticsFunctions {ext : ffi_syntax} :=
     load : go.type → val;
     store : go.type → val;
 
-    struct_field_ref : go.type → go_string → loc → loc;
+    (* This uses a Gallina [Type] because there are multiple [go.type]s that
+       have the same [Type] representation (e.g. uint64/int64, *X/*Y), but
+       offsets are only supposed to depend on the Gallina representation. *)
+    is_type_repr : go.type → Type → Prop;
+    struct_field_ref : Type → go_string → loc → loc;
+
     struct_field_get : go.type → go_string → val → expr;
     struct_field_set : go.type → go_string → val → val → expr;
 
@@ -90,7 +95,7 @@ Class GoSemanticsFunctions {ext : ffi_syntax} :=
        expression. https://go.dev/ref/spec#Index_expressions *)
     index (container_type : go.type) (i : Z) (v : val) : expr;
     index_ref (container_type : go.type) (i : Z) (v : val) : expr;
-    array_index_ref (elem_type : go.type) (i : Z) (l : loc) : loc;
+    array_index_ref (elem_type : Type) (i : Z) (l : loc) : loc;
 
     map_empty : val → val;
     map_lookup : val → val → bool * val;
@@ -148,7 +153,7 @@ Inductive is_primitive_zero_val : go.type → val → Prop :=
 Global Instance interface_eq_dec : EqDecision interface.t.
 Proof. solve_decision. Qed.
 
-Global Instance array_eq_dec t V n `{!EqDecision V} : EqDecision (array.t t V n).
+Global Instance array_eq_dec V n `{!EqDecision V} : EqDecision (array.t V n).
 Proof. solve_decision. Qed.
 
 Global Instance func_eq_dec : EqDecision func.t.
@@ -301,6 +306,12 @@ Class Underlying t tunder  `{!GoSemanticsFunctions} : Prop :=
     to_underlying_unfold : to_underlying t = tunder
   }.
 
+Class TypeRepr `{!GoSemanticsFunctions} t V : Prop :=
+  {
+    type_repr : is_type_repr t V;
+  }.
+Global Hint Mode TypeRepr - ! - : typeclass_instances.
+
 (** [go.CoreSemantics] defines the basics of when a GoContext is valid,
     excluding predeclared types (including primitives), arrays, slice, map, and
     channels, each of which is in their own file.
@@ -319,7 +330,8 @@ Class CoreSemantics :=
   #[global] go_func_resolve_step n ts :: IsGoStepPureDet (FuncResolve n ts) #() #(functions n ts);
   #[global] go_method_resolve_step m t :: IsGoStepPureDet (MethodResolve t m) #() #(methods t m);
   #[global] go_global_var_addr_step v :: IsGoStepPureDet (GlobalVarAddr v) #() #(global_addr v);
-  #[global] struct_field_ref_step t f l :: IsGoStepPureDet (StructFieldRef t f) #l #(struct_field_ref t f l);
+  #[global] struct_field_ref_step t f l V `{!TypeRepr t V} ::
+    IsGoStepPureDet (StructFieldRef t f) #l #(struct_field_ref V f l);
   #[global] go_interface_make_step t v :: IsGoStepPureDet (InterfaceMake t) v #(interface.mk t v);
   #[global] composite_literal_step t (v : val) :: IsGoStepPureDet (CompositeLiteral t) v (composite_literal t v);
   go_prealloc_step : is_go_step_pure GoPrealloc #() = (λ e, ∃ (l : loc), e = #l);
@@ -396,7 +408,6 @@ Class CoreSemantics :=
                 GoStore field_type (field_addr, field_val)
          ) (GoZeroVal (go.StructType fds) #()) fds)%V;
 
-  struct_field_ref_underlying `{!Underlying t t'} : struct_field_ref t = struct_field_ref t';
   index_ref_underlying `{!Underlying t t'} : index_ref t = index_ref t';
   index_underlying `{!Underlying t t'} : index t = index t';
 
